Batteries/Data/Fin/Lemmas.lean
@@ -100,7 +100,7 @@ theorem foldl_succ_last (f : α → Fin (n+1) → α) (x) :
     foldl (n+1) f x = f (foldl n (f · ·.castSucc) x) (last n) := by
   rw [foldl_succ]
   induction n generalizing x with
-  | zero => simp [foldl_succ, Fin.last]
+  | zero => simp [foldl_succ, last]
   | succ n ih => rw [foldl_succ, ih (f · ·.succ), foldl_succ]; simp [succ_castSucc]
 
 theorem foldl_eq_foldlM (f : α → Fin n → α) (x) :
@@ -131,7 +131,7 @@ theorem foldr_succ (f : Fin (n+1) → α → α) (x) :
 theorem foldr_succ_last (f : Fin (n+1) → α → α) (x) :
     foldr (n+1) f x = foldr n (f ·.castSucc) (f (last n) x) := by
   induction n generalizing x with
-  | zero => simp [foldr_succ, Fin.last]
+  | zero => simp [foldr_succ, last]
   | succ n ih => rw [foldr_succ, ih (f ·.succ), foldr_succ]; simp [succ_castSucc]
 
 theorem foldr_eq_foldrM (f : Fin n → α → α) (x) :
@@ -149,3 +149,96 @@ theorem foldr_rev (f : α → Fin n → α) (x) :
   induction n generalizing x with
   | zero => simp
   | succ n ih => rw [foldl_succ_last, foldr_succ, ← ih]; simp [rev_succ]
+
+/-! ### foldM -/
+
+variable {n : Nat} {α : Fin (n+1) → Type _} [Monad m]
+    (f : ∀ (i : Fin n), α i.castSucc → m (α i.succ))
+
+theorem foldM_loop_lt (h : i < n) (x : α ⟨i, Nat.lt_add_right 1 h⟩) :
+    foldM.loop n α f i (Nat.lt_add_right 1 h) x =
+      (f ⟨i, h⟩ x) >>= (foldM.loop n α f (i+1) (Nat.add_lt_add_right h 1)) := by
+  rw [foldM.loop, dif_pos h]
+
+theorem foldM_loop_eq (x : α ⟨n, Nat.le_refl _⟩) :
+    foldM.loop n α f n (Nat.le_refl _) x = pure x := by
+  rw [foldM.loop, dif_neg (Nat.lt_irrefl _), cast_eq]
+
+@[simp] theorem foldM_zero {α : Fin 1 → Sort _} (f : (i : Fin 0) → α i.castSucc → m (α i.succ))
+    (x : α 0) : foldM 0 α f x = pure x :=
+  foldM_loop_eq ..
+
+variable {α : Fin (n+2) → Type _} (f : (i : Fin (n+1)) → α i.castSucc → m (α i.succ))
+
+theorem foldM_loop (h : i < n+1) (x : α ⟨i, Nat.lt_add_right 1 h⟩) :
+    foldM.loop (n+1) α f i (Nat.lt_add_right 1 h) x =
+      f ⟨i, h⟩ x >>= (foldM.loop n (α ∘ succ) (f ·.succ ·) i h .) := by
+  if h' : i < n then
+    rw [foldM_loop_lt _ h _]
+    congr; funext
+    rw [foldM_loop_lt _ h' _, foldM_loop]; rfl
+  else
+    cases Nat.le_antisymm (Nat.le_of_lt_succ h) (Nat.not_lt.1 h')
+    rw [foldM_loop_lt]
+    congr; funext
+    rw [foldM_loop_eq, foldM_loop_eq]
+
+theorem foldM_succ (x) : foldM (n+1) α f x = f 0 x >>= foldM n (α ∘ succ) (f ·.succ ·) :=
+  foldM_loop ..
+
+/-- Dependent version `foldM` equals non-dependent version `foldlM` --/
+theorem foldM_eq_foldlM {α : Type _} (f : Fin n → α → m α) (x : α) :
+    foldM n (fun _ => α) f x = foldlM n (fun x i => f i x) x := by
+  induction n generalizing x with
+  | zero => simp only [foldM_zero, foldlM_zero]
+  | succ n ih =>
+    simp only [foldM_succ, foldlM_succ, Function.comp_apply, Function.comp_def]
+    congr; ext; simp only [ih]
+
+/-! ### fold -/
+
+variable {α : Fin (n+1) → Sort _} (f : ∀ (i : Fin n), α i.castSucc → α i.succ)
+
+theorem fold_loop_lt (h : i < n) (x : α ⟨i, Nat.lt_add_right 1 h⟩) :
+    fold.loop n α f i (Nat.lt_add_right 1 h) x =
+      fold.loop n α f (i+1) (Nat.add_lt_add_right h 1) (f ⟨i, h⟩ x) := by
+  rw [fold.loop, dif_pos h]
+
+theorem fold_loop_eq (x : α ⟨n, Nat.le_refl _⟩) :
+    fold.loop n α f n (Nat.le_refl _) x = x := by
+  rw [fold.loop, dif_neg (Nat.lt_irrefl _), cast_eq]
+
+@[simp] theorem fold_zero {α : Fin 1 → Sort _} (f : (i : Fin 0) → α i.castSucc → α i.succ)
+    (x : α 0) : fold 0 α f x = x :=
+  fold_loop_eq ..
+
+variable {α : Fin (n+2) → Sort _} (f : (i : Fin (n+1)) → α i.castSucc → α i.succ)
+
+theorem fold_loop (h : i < n+1) (x : α ⟨i, Nat.lt_add_right 1 h⟩) :
+    fold.loop (n+1) α f i (Nat.lt_add_right 1 h) x =
+      fold.loop n (α ∘ succ) (f ·.succ ·) i h (f ⟨i, h⟩ x) := by
+  if h' : i < n then
+    rw [fold_loop_lt _ h _]
+    rw [fold_loop_lt _ h' _, fold_loop]; rfl
+  else
+    cases Nat.le_antisymm (Nat.le_of_lt_succ h) (Nat.not_lt.1 h')
+    rw [fold_loop_lt]
+    rw [fold_loop_eq, fold_loop_eq]
+
+theorem fold_succ (x : α 0) : fold (n+1) α f x = fold n (α ∘ succ) (f ·.succ ·) (f 0 x) :=
+  fold_loop ..
+
+theorem fold_succ_last (x : α 0) :
+    fold (n+1) α f x = f (last n) (fold n (α ∘ castSucc) (f ·.castSucc ·) x) := by
+  rw [fold_succ]
+  induction n with
+  | zero => simp [fold_succ, last]
+  | succ n ih => rw [fold_succ, @ih (α ∘ succ) (f ·.succ ·), fold_succ]; congr
+
+theorem fold_eq_foldl {α : Sort _} (f : Fin n → α → α) (x : α) :
+    fold n (fun _ => α) f x = foldl n (fun x i => f i x) x := by
+  induction n generalizing x with
+  | zero => simp only [fold_zero, foldl_zero]
+  | succ n ih =>
+    simp only [fold_succ, foldl_succ, Function.comp_apply, Function.comp_def]
+    congr; simp only [ih]
